Finished the agreement proof!

Isabelle2/Paxos.thy
@@ -5,19 +5,7 @@ imports "/home/nano/Documents/IO-Automata/IOA_Automation"  "~~/src/HOL/Eisbach/E
   Transfer
 begin
 
-datatype ('v,'acc,'l, 'b::linorder) p_action =
-  Propose 'v
-| Learn 'v 'l
-| Vote 'acc
-| JoinBallot 'b 'acc
-
-(* TODO: using 'b::linorder confuses the record package. *)
-record ('v, 'acc, 'b) p_state =
-  propCmd :: "'v fset"
-  ballot :: "'acc \<Rightarrow> 'b option"
-  vote :: "'acc \<Rightarrow> 'b \<Rightarrow> 'v option"
-  suggestion :: "'b \<Rightarrow> 'v option"
-    -- {* The suggestion of the leader of round b *}
+section {* nat option as a linear order *}
 
 fun less_eq_o where 
   "less_eq_o None _ = True"
@@ -29,37 +17,6 @@ fun less_o where
 | "less_o None _ = True"
 | "less_o (Some x) None = False"
 | "less_o (Some x) (Some y) = (x < y)"
-
-subsection {* Transfer between nat option and nat *}
-
-interpretation lifting_syntax .
-
-fun nno where 
-  "nno (x::nat) None = (x = 0)"
-| "nno x (Some y) = (x = Suc y)"
-
-lemma zero_None_trans[transfer_rule]:"nno (0::nat) None"
-by (auto simp add:rel_fun_def)
-
-lemma less_trans[transfer_rule]:"(nno ===> nno ===> (op \<longleftrightarrow>)) ((op \<le>)::nat \<Rightarrow> nat \<Rightarrow> bool) less_eq_o"
-apply(auto simp add:rel_fun_def)
-apply (metis Suc_le_mono antisym_conv2 le_0_eq less_eq_o.elims(3) option.discI option.inject nno.elims(2) zero_less_Suc)
-by (metis Suc_le_mono eq_iff less_eq_o.elims(2) less_imp_le_nat option.discI option.inject nno.elims(2) zero_less_Suc)
-
-lemma all_trans[transfer_rule]: "((nno ===> (op \<longleftrightarrow>)) ===> (op \<longleftrightarrow>)) All All"
-apply(auto simp add:rel_fun_def)
-apply (metis split_option_all nno.simps(1) nno.simps(2))
-by (metis nat_induct nno.simps(1) nno.simps(2))
-
-text {* Test of transfer *}
-lemma haha[rule_format]: "\<forall> y . less_eq_o None (y::nat option)"
-apply transfer_start
-apply transfer_step
-apply transfer_step
-apply transfer_step
-apply transfer_end
-apply auto
-done
 
 instantiation option :: (linorder) linorder
 begin
@@ -80,22 +37,39 @@ by (metis le_cases less_eq_o.elims(3) option.discI option.inject)
 
 end
 
-class linorder_bot = linorder + order_bot
+section {* State and actions of the Paxos algorithm *}
+
+datatype ('v,'acc,'l) p_action =
+  Propose 'v
+| Learn 'v 'l
+| Vote 'acc
+| JoinBallot nat 'acc
+| StartBallot nat
+
+(* Note: using 'b::linorder confuses the record package. *)
+record ('v, 'acc, 'b) p_state =
+  propCmd :: "'v fset"
+  ballot :: "'acc \<Rightarrow> 'b option"
+  vote :: "'acc \<Rightarrow> 'b \<Rightarrow> 'v option"
+  suggestion :: "'b \<Rightarrow> 'v option"
+    -- {* The suggestion of the leader of round b *}
+
+section {* Properties of the state *}
 
 locale Paxos = IOA +
   fixes acceptors::"'acc fset" and learners::"'l fset" and quorums::"'acc fset fset"
-  (*and max::"('b::linorder) set \<Rightarrow> 'b"*)
   assumes "acceptors \<noteq> {||}"
     and "learners \<noteq> {||}"
     and "\<And> q1 q2 . \<lbrakk>q1 |\<in>| quorums; q2 |\<in>| quorums\<rbrakk> \<Longrightarrow> q1 |\<inter>| q2 \<noteq> {||}"
     and "\<And> q . q |\<in>| quorums \<Longrightarrow> q |\<subseteq>| acceptors"
-    and "quorums \<noteq> {||}" (*
-    and "\<And> bs . finite bs \<Longrightarrow> max bs \<in> bs"
-    and "\<And> b bs . \<lbrakk>finite bs; b \<in> bs\<rbrakk> \<Longrightarrow> b \<le> max bs"*)
+    and "quorums \<noteq> {||}"
 begin
 
 text {* If Nitpick can find a model then the assumptions are not contradictory *}
 lemma False nitpick oops
+
+text {* A state is conservative when for every ballot b: if a1 and a2 have voted in b, 
+  then their vote is the same *}
 
 definition conservative where
   "conservative r b \<equiv> \<forall> a1 . \<forall> a2 . a1 |\<in>| acceptors \<and> a2 |\<in>| acceptors \<longrightarrow> (
@@ -105,53 +79,16 @@ definition conservative where
 definition conservative_array where
   "conservative_array r \<equiv> \<forall> b . conservative r b"
 
-fun max_vote_2 where
-  "max_vote_2 votes (0::nat) = votes 0 \<bind> (\<lambda> v . Some (0,v))"
-| "max_vote_2 votes (Suc b) = 
-    ( case (votes (Suc b)) of None \<Rightarrow> max_vote_2 votes b
-      |  Some v \<Rightarrow> Some (Suc b, v) )"
-
-lemma assumes "i \<le> b" and "votes i \<noteq> None"
-  shows "case (max_vote_2 votes b) of None \<Rightarrow> False | Some (m,v) \<Rightarrow> i \<le> m"
-using assms
-proof (induct votes b rule:max_vote_2.induct)
-  case 1 thus ?case by fastforce
-next
-  case 2 thus ?case by auto (metis case_prodI le_Suc_eq option.case_eq_if option.sel option.simps(3))
-qed
-
-declare option.split[split]
-
-lemma
-  "case (max_vote_2 votes b) of None \<Rightarrow> True | Some (m,v) \<Rightarrow> m \<le> b \<and> votes m = Some v"
-proof (induct votes b rule:max_vote_2.induct)
-case (1 votes) thus ?case 
-  apply (auto)
-    apply (metis (no_types, lifting) Pair_inject bind_eq_Some_conv option.inject)
-  apply (smt bind_eq_Some_conv option.sel prod.inject)
-  done
-next
-  case (2 votes b) thus ?case by auto
-qed
-
 text {* Here the max is the one from Lattices_Big *}
 
-definition max_acc_voted_round where
-  "max_acc_voted_round r a bound \<equiv> Max {b . vote r a b \<noteq> None \<and> b \<le> bound}"
-  
 definition max_voted_round where
-  "max_voted_round r q bound \<equiv> Max {max_acc_voted_round r a bound | a . a |\<in>| q}"
+  "max_voted_round r a bound \<equiv> Max {b . vote r a b \<noteq> None \<and> b \<le> bound}"
   
-definition max_voted_round_2 where
-  "max_voted_round_2 r q bound \<equiv> 
+definition max_voted_round_q where
+  "max_voted_round_q r q bound \<equiv> 
     if \<exists> b a . a |\<in>| q \<and> b \<le> bound \<and> vote r a b \<noteq> None
     then Some (Max {b . \<exists> a . a |\<in>| q \<and> b \<le> bound \<and> vote r a b \<noteq> None})
     else None"
-
-lemma assumes "n > Max {j . P j}"
-  and "finite {j . P j}"
-  shows "\<not> P n" using assms
-  by (metis Max_ge mem_Collect_eq not_le)
 
 lemma finite_voted_bals:"finite {b::nat . \<exists> a . a |\<in>| q \<and> b \<le> bound \<and> vote r a b \<noteq> None}"
 proof -
@@ -164,42 +101,42 @@ qed
 
 lemma max_voted_round_none:
   assumes "a |\<in>| q" and "(b::nat) \<le> bound" 
-  and "max_voted_round_2 r q bound = None \<or> b > the (max_voted_round_2 r q bound)"
+  and "max_voted_round_q r q bound = None \<or> b > the (max_voted_round_q r q bound)"
   shows "vote r a b = None"
-proof (cases "max_voted_round_2 r q bound")
+proof (cases "max_voted_round_q r q bound")
 case None 
   thus ?thesis using assms(1,2)
-  by (auto simp add:max_voted_round_2_def split:split_if_asm)
+  by (auto simp add:max_voted_round_q_def split:split_if_asm)
 next
   case (Some b\<^sub>m\<^sub>a\<^sub>x)
   with this obtain a2 b2 v where "a2 |\<in>| q \<and> b2 \<le> bound \<and> vote r a2 b2 = Some v"
-  by (auto simp add:max_voted_round_2_def split:split_if_asm)
+  by (auto simp add:max_voted_round_q_def split:split_if_asm)
   hence "{b . \<exists> a . a |\<in>| q \<and> b \<le> bound \<and> vote r a b \<noteq> None} \<noteq> {}" by auto
   with this obtain b2 a2 where "a2 |\<in>| q \<and> b2 \<le> bound \<and> vote r a2 b2 \<noteq> None"
     by auto
   moreover note finite_voted_bals
   moreover have "b > Max {b . \<exists> a . a |\<in>| q \<and> b \<le> bound \<and> vote r a b \<noteq> None}" using Some assms(3)
-    by (auto simp add:max_voted_round_2_def split:split_if_asm)
+    by (auto simp add:max_voted_round_q_def split:split_if_asm)
   ultimately
   show ?thesis by (metis (mono_tags, lifting) Max.coboundedI assms(1,2) leD mem_Collect_eq) 
 qed
 
 lemma max_voted_round_some :
-  assumes "max_voted_round_2 r q (bound::nat) = Some (b::nat)"
+  assumes "max_voted_round_q r q (bound::nat) = Some (b::nat)"
   obtains a where "a |\<in>| q" and "vote r a b \<noteq> None" and "b \<le> bound"
 proof -
   from assms have "b = Max {b . \<exists> a . a |\<in>| q \<and> b \<le> bound \<and> vote r a b \<noteq> None}"
-    by (auto simp add:max_voted_round_2_def split:split_if_asm)
+    by (auto simp add:max_voted_round_q_def split:split_if_asm)
   moreover note finite_voted_bals
   moreover obtain a2 b2 where "a2 |\<in>| q \<and> b2 \<le> bound \<and> vote r a2 b2 \<noteq> None"
-    using assms by (auto simp add:max_voted_round_2_def) (metis option.distinct(1))
+    using assms by (auto simp add:max_voted_round_q_def) (metis option.distinct(1))
   ultimately show ?thesis using that
   by (smt Max_in empty_iff finite_nat_set_iff_bounded_le mem_Collect_eq) 
 qed
  
 definition max_vote where
   "max_vote r q bound \<equiv>
-    case max_voted_round_2 r q bound of
+    case max_voted_round_q r q bound of
       None \<Rightarrow> None
     | Some b \<Rightarrow> 
         let max_voter = (SOME a . a |\<in>| q \<and> vote r a b \<noteq> None)
@@ -211,7 +148,7 @@ lemma max_vote_some_prop:
   and "\<And> a2 b2 . \<lbrakk>a2 |\<in>| q; b2 > b\<^sub>m\<^sub>a\<^sub>x; b2 \<le> bound\<rbrakk> \<Longrightarrow> vote r a2 b2 = None"
   and "b\<^sub>m\<^sub>a\<^sub>x \<le> bound"
 proof -
-  from assms obtain b\<^sub>m\<^sub>a\<^sub>x where 0:"max_voted_round_2 r q bound = Some (b\<^sub>m\<^sub>a\<^sub>x::nat)"
+  from assms obtain b\<^sub>m\<^sub>a\<^sub>x where 0:"max_voted_round_q r q bound = Some (b\<^sub>m\<^sub>a\<^sub>x::nat)"
     by (auto simp add:max_vote_def) (metis (lifting) not_None_eq option.simps(4)) 
   with max_voted_round_some obtain a where
     "a |\<in>| q" and "vote r a b\<^sub>m\<^sub>a\<^sub>x \<noteq> None" and 1:"b\<^sub>m\<^sub>a\<^sub>x \<le> bound" by metis
@@ -266,7 +203,7 @@ definition well_formed where
   "well_formed r \<equiv> \<forall> a b . a |\<in>| acceptors \<and> (ballot r) a < b  
     \<longrightarrow> (vote r) a (the b) = None"
 
-lemma "safe_at r v (bot::'a::linorder_bot)"
+lemma "safe_at r v (bot::nat)"
 by (auto simp add:safe_at_def)
 
 lemma chosen_at_is_choosable:
@@ -349,19 +286,22 @@ proof -
   ultimately show ?thesis by fastforce
 qed
 
-lemma proved_safe:
+text {* The main lemma *}
+
+lemma proved_safe_is_safe:
   assumes "safe s" and "q |\<in>| quorums"
   and "\<And> a . a |\<in>| q \<Longrightarrow> ballot s a \<ge> Some i"
-  and "proved_safe_at s q i v"
+  and "proved_safe_at s q i v" and "conservative_array s"
   shows "safe_at s v (i::nat)"
 proof (cases "i = 0")
   case True thus ?thesis
     by (metis not_less0 safe_at_def) 
 next
   case False
-  consider (a) k a
-    where "a |\<in>| q" and "vote s a k = Some v" and "k < i"
-    and "\<And> a\<^sub>2 l . \<lbrakk>a\<^sub>2 |\<in>| q; k < l; l < i\<rbrakk> \<Longrightarrow> vote s a\<^sub>2 l = None"
+  consider 
+    (a) k a
+      where "a |\<in>| q" and "vote s a k = Some v" and "k < i"
+      and "\<And> a\<^sub>2 l . \<lbrakk>a\<^sub>2 |\<in>| q; k < l; l < i\<rbrakk> \<Longrightarrow> vote s a\<^sub>2 l = None"
   | (b) "\<And> a k . \<lbrakk>a |\<in>| q; k < i\<rbrakk>  \<Longrightarrow> vote s a k = None"
   proof (cases "max_vote s q (i-1)")
     case None 
@@ -379,7 +319,7 @@ next
   qed
   thus ?thesis
   proof (cases)
-    case b 
+    case b
     { fix j v
       assume 1:"j < i"  and 2:"choosable s v j"
       from 2 obtain q2 where 3:"q2 |\<in>| quorums" and 4:"\<And> a . a |\<in>| q2 \<Longrightarrow>
@@ -387,10 +327,8 @@ next
         by (auto simp add:choosable_def)
       from 3 assms(2) obtain a where 5:"a |\<in>| q" and 6:"a |\<in>| q2"
         using quorum_inter_witness by metis
-      have 8:"ballot s a \<ge> Some j" using assms(3)
-        by (metis "1" "5" less_eq_def less_eq_o.simps(3) less_imp_le order_trans) 
-      have 9:"vote s a j = Some v" using assms(3)
-        by (metis "1" "4" "5" "6" "8" leD le_neq_trans less_eq_def less_eq_o.simps(3))
+      have 9:"vote s a j = Some v"
+        by (metis (no_types, hide_lams) "1" "4" "5" "6" assms(3) less_def less_o.simps(4) not_le order_trans) 
       from b have False by (metis "1" "5" "9" option.distinct(1)) }
     thus ?thesis by (auto simp add:safe_at_def)
   next
@@ -400,45 +338,45 @@ next
       consider (aa) "j < k" | (bb) "j = k" | (cc) "k < j" by fastforce
       hence ?thesis
       proof cases
-      case aa
-      have "a |\<in>| acceptors"
-        by (metis Paxos_axioms Paxos_def a(1) assms(2) fset_mp) 
-      hence "safe_at s v k" using  assms(1)
-        by (metis a(2) option.discI option.sel safe_def)
-      with aa show ?thesis using that by (metis safe_at_def) 
-    next
-      case cc
-      from that obtain q2 where 3:"q2 |\<in>| quorums" and 4:"\<And> a . a |\<in>| q2 \<Longrightarrow>
-        (ballot s a) > Some j \<Longrightarrow> (vote s) a j = Some v'"
-        by (auto simp add:choosable_def)
-      from 3 assms(2) obtain a2 where 5:"a2 |\<in>| q" and 6:"a2 |\<in>| q2" 
-        using quorum_inter_witness by metis
-      from 5 assms(3) that(2) have 7:"ballot s a2 \<ge> Some j"
-        by (metis less_eq_def less_eq_o.simps(3) less_imp_le order_trans) 
-      from 7 6 4 have 8:"vote s a2 j = Some v'"
-        by (metis "5" antisym_conv2 assms(3) leD less_eq_def less_eq_o.simps(3) that(2)) 
-      show ?thesis using a(4) 5 that(2) 8 cc by (metis option.distinct(1))
-    next
-      case bb (* Here we probably need the fact that the array is conservative: *)
-      have 1:"\<And> a . a |\<in>| acceptors \<Longrightarrow> vote s a k = Some v" sorry
-      from that obtain q2 where 3:"q2 |\<in>| quorums" and 4:"\<And> a . a |\<in>| q2 \<Longrightarrow>
-        (ballot s a) > Some j \<Longrightarrow> (vote s) a j = Some v'"
-        by (auto simp add:choosable_def)
-      from 3 assms(2) obtain a2 where 5:"a2 |\<in>| q" and 6:"a2 |\<in>| q2" 
-        using quorum_inter_witness by metis
-      have 7:"ballot s a2 \<ge> Some k"
-        by (metis "5" a(3) assms(3) less_eq_def less_eq_o.simps(3) less_imp_le order_trans)
-      have 8:"a2 |\<in>| acceptors"
-        by (metis "5" Paxos_axioms Paxos_def assms(2) order.not_eq_order_implies_strict pfsubsetD) 
-      have 9:"vote s a2 k = Some v"
-        by (metis "1" "8")
-      show ?thesis
-        by (metis "4" "5" "6" "7" "9" antisym_conv2 assms(3) bb leD less_eq_def less_eq_o.simps(3) option.sel that(2)) 
+        case aa
+        have "a |\<in>| acceptors"
+          by (metis Paxos_axioms Paxos_def a(1) assms(2) fset_mp) 
+        hence "safe_at s v k" using  assms(1)
+          by (metis a(2) option.discI option.sel safe_def)
+        with aa show ?thesis using that by (metis safe_at_def) 
+      next
+        case cc
+        from that obtain q2 where 3:"q2 |\<in>| quorums" and 4:"\<And> a . a |\<in>| q2 \<Longrightarrow>
+          (ballot s a) > Some j \<Longrightarrow> (vote s) a j = Some v'"
+          by (auto simp add:choosable_def)
+        from 3 assms(2) obtain a2 where 5:"a2 |\<in>| q" and 6:"a2 |\<in>| q2" 
+          using quorum_inter_witness by metis
+        have 8:"vote s a2 j = Some v'"
+          by (metis (mono_tags, lifting) "4" "5" "6" assms(3) leD leI less_eq_def less_eq_o.simps(3) order_trans that(2)) 
+        show ?thesis using a(4) 5 that(2) 8 cc by (metis option.distinct(1))
+      next
+        case bb (* Here we probably need the fact that the array is conservative: *)
+        have 1:"vote s a k = Some v" if "a |\<in>| acceptors" and " vote s a k \<noteq> None"  for a using that assms(5) 
+          by (auto simp add:conservative_array_def conservative_def)
+            (metis (no_types, hide_lams) Paxos_axioms Paxos_def a(1) a(2) assms(2) option.inject order.not_eq_order_implies_strict pfsubsetD)  
+        from that obtain q2 where 3:"q2 |\<in>| quorums" and 4:"\<And> a . a |\<in>| q2 \<Longrightarrow>
+          (ballot s a) > Some j \<Longrightarrow> (vote s) a j = Some v'"
+          by (auto simp add:choosable_def)
+        from 3 assms(2) obtain a2 where 5:"a2 |\<in>| q" and 6:"a2 |\<in>| q2" 
+          using quorum_inter_witness by metis
+        have 7:"ballot s a2 \<ge> Some k"
+          by (metis "5" a(3) assms(3) less_eq_def less_eq_o.simps(3) less_imp_le order_trans)
+        have 8:"a2 |\<in>| acceptors"
+          by (metis "5" Paxos_axioms Paxos_def assms(2) order.not_eq_order_implies_strict pfsubsetD) 
+        have 9:"vote s a2 k = Some v"
+          by (metis "1" "4" "5" "6" "7" "8" assms(3) bb leD less_eq_def less_eq_o.simps(3) option.discI order.not_eq_order_implies_strict that(2))
+        show ?thesis
+          by (metis "4" "5" "6" "7" "9" antisym_conv2 assms(3) bb leD less_eq_def less_eq_o.simps(3) option.sel that(2)) 
+      qed
+      thus ?thesis by (auto simp add:safe_at_def)
     qed
-    thus ?thesis by (auto simp add:safe_at_def)
-  qed
-  thus ?thesis
-  by (metis Paxos.safe_at_def Paxos_axioms) 
+    thus ?thesis
+    by (metis Paxos.safe_at_def Paxos_axioms) 
   qed 
 qed
   
@@ -459,11 +397,11 @@ definition propose where
   "propose c r r' \<equiv> (r' = r\<lparr>propCmd := (propCmd r) |\<union>| {|c|}\<rparr>)"
 
 definition join_ballot where
-  "join_ballot a b s s' \<equiv> b > (ballot s a) \<and> s' = s\<lparr>ballot := (ballot s)(a := b)\<rparr>"
+  "join_ballot a b s s' \<equiv> Some b > (ballot s a) \<and> s' = s\<lparr>ballot := (ballot s)(a := Some b)\<rparr>"
 
 definition start_ballot where
   "start_ballot b s s' \<equiv> suggestion s b = None \<and>
-    (\<exists> q v . q |\<in>| quorums \<and> proved_safe_at s q b v
+    (\<exists> q v . q |\<in>| quorums \<and> proved_safe_at s q b v \<and> (\<forall> a . a |\<in>| q \<longrightarrow> ballot s a \<ge> Some b)
       \<and> v |\<in>| propCmd s \<and> s' = s\<lparr>suggestion := (suggestion s)(b := Some v)\<rparr>)"
 
 definition do_vote where
@@ -478,6 +416,7 @@ fun p_trans_fun  where
 | "p_trans_fun r (JoinBallot b a) r' = join_ballot a b r r'"
 | "p_trans_fun r (Vote a) r' = do_vote a r r'"
 | "p_trans_fun r (Learn v l) r' = learn l v r r'"
+| "p_trans_fun r (StartBallot b) r' = start_ballot b r r'"
 
 definition p_trans where
   "p_trans \<equiv> { (r,a,r') . p_trans_fun r a r'}"
@@ -486,6 +425,8 @@ definition p_ioa where
   "p_ioa \<equiv> \<lparr>ioa.asig = p_asig, start = p_start, trans = p_trans\<rparr>"
 
 end 
+
+section {* Correctness proof *}
 
 text {* We create a locale for the proof in order to fix the type variables appearing in p_ioa_def
   Otherwise we run into problem with polymorphism and Eisbach *}
@@ -506,7 +447,7 @@ lemma gt_not_none:
 by (metis less_def less_o.elims(2) option.discI)
 
 declare propose_def[simp] join_ballot_def[simp] do_vote_def[simp]
-  learn_def[simp]
+  learn_def[simp] start_ballot_def[simp]
 
 definition inv1 where
   "inv1 s \<equiv> \<forall> a b . a |\<in>| acceptors \<and> vote s a b \<noteq> None 
@@ -518,9 +459,10 @@ declare the_ioa_def[inv_proofs_defs]
 lemma inv1:"invariant the_ioa inv1"
 apply try_solve_inv2
 apply (smt fun_upd_apply p_state.ext_inject p_state.surjective p_state.update_convs(3))
+apply (metis (no_types, lifting) map_upd_Some_unfold option.discI p_state.ext_inject p_state.surjective p_state.update_convs(4))
 done
-declare inv1[invs]
 
+(* Does not seem needed. Is it? *)
 declare well_formed_def[inv_proofs_defs]
 lemma well_formed_inductive:
   "invariant the_ioa well_formed"
@@ -528,18 +470,178 @@ apply try_solve_inv2
 apply auto
 apply (smt fun_upd_apply gt_not_none neq_iff option.collapse option.sel p_state.ext_inject p_state.surjective p_state.update_convs(3))
 done
-declare well_formed_inductive[invs]
+(*declare well_formed_inductive[invs]*)
 
 declare conservative_array_def[inv_proofs_defs]
 lemma conservative_inductive:
   "invariant the_ioa conservative_array"
-apply (try_solve_inv2 inv_proofs_defs:inv_proofs_defs conservative_def)
+apply (try_solve_inv2 inv_proofs_defs:inv_proofs_defs conservative_def invs:invs inv1)
+apply metis
 apply metis
 done
+declare conservative_inductive[invs]
 
-lemma 
-  "\<lbrakk>reachable p_ioa s; chosen s v\<^sub>1; chosen s v\<^sub>2\<rbrakk> \<Longrightarrow> v\<^sub>1 = v\<^sub>2 " oops
+lemma safe_mono:
+  assumes "safe_at s v b" and "s \<midarrow>a\<midarrow>the_ioa\<longrightarrow> t"
+  shows "safe_at t v b" using assms
+apply (cases a)
+        apply (auto simp add:inv_proofs_defs safe_at_def choosable_def)[2] (* propose, learn *)
+    defer (* join_ballot *)
+    apply (simp add:inv_proofs_defs safe_at_def choosable_def)[1]
+    apply (metis less_def order.strict_trans) 
+  defer (* vote *)
+  apply (simp add:inv_proofs_defs safe_at_def choosable_def)
+  apply (smt fun_upd_apply neq_iff option.sel p_state.select_convs(2) p_state.select_convs(3) p_state.surjective p_state.update_convs(3))
+  (* That was amazing, Sledgehammer found it before I had time to think about why it would be true... *)
+  (* Something may be wrong, I would have expected this to be much harder... *)
+apply (simp add:inv_proofs_defs safe_at_def choosable_def) (* start_ballot *)
+apply (metis p_state.ext_inject p_state.surjective p_state.update_convs(4))
+done
+
+definition inv2 where
+  "inv2 s \<equiv> safe s \<and> (\<forall> b . case suggestion s b of None \<Rightarrow> True | Some v \<Rightarrow> safe_at s v b)"
+
+declare inv2_def[inv_proofs_defs]
+
+lemma inv2:
+  "invariant the_ioa inv2"
+apply(rule invariantI)
+    apply (force simp add:inv_proofs_defs safe_def)
+  apply instantiate_invs_2
+  apply (case_tac a)
+          subgoal premises prems for s t a v
+          proof -
+            from prems(2,5) have 1:"propose v s t"
+              by(auto simp add:inv_proofs_defs) 
+            hence 2:"\<And> b . suggestion s b = suggestion t b" 
+              by(auto simp add:inv_proofs_defs)
+            have 3:"safe t" using 1 prems(1) 
+              by (auto simp add:inv_proofs_defs safe_def safe_at_def choosable_def) 
+            from 1 2 3 safe_mono show ?thesis 
+              by (auto simp add:inv2_def)
+                (metis inv2_def option.case_eq_if prems(1) prems(2))
+          qed
+        subgoal by (auto simp add:inv_proofs_defs) (* learn *)
+      subgoal premises prems for s t act a
+      proof - 
+        from prems(2,5) have 1:"do_vote a s t"
+          by(auto simp add:inv_proofs_defs)
+        hence 2:"\<And> b . suggestion s b = suggestion t b" 
+          by (auto simp add:inv_proofs_defs)
+            (metis p_state.ext_inject p_state.surjective p_state.update_convs(3))
+        have 3:"safe t" using prems(1) 1 apply(auto simp add:inv2_def safe_def)
+        proof - (* Auto-generated *)
+          fix b :: nat and aa :: 'a
+          assume a1: "let bo = ballot s a; b = the bo in (\<exists>y. bo = Some y) \<and> vote s a b = None \<and> t = s \<lparr>vote := (vote s)(a := (vote s a)(b := suggestion s b))\<rparr>"
+          assume a2: "\<forall>b a. a |\<in>| acceptors \<longrightarrow> (let vote = vote s a b in (\<exists>y. vote = Some y) \<longrightarrow> safe_at s (the vote) b)"
+          assume a3: "\<forall>b. case suggestion s b of None \<Rightarrow> True | Some v \<Rightarrow> safe_at s v b"
+          assume a4: "aa |\<in>| acceptors"
+          { fix cc :: 'c
+            have ff1: "\<forall>p. \<exists>f fa fb fc u. p = \<lparr>propCmd = f::'c fset, ballot = fa::'a \<Rightarrow> nat option, vote = fb, suggestion = fc, \<dots> = u::unit\<rparr>"
+              by (metis p_state.cases_scheme)
+            obtain nn :: nat where
+              ff2: "ballot s a = Some nn \<and> vote s a (the (ballot s a)) = None \<and> t = s \<lparr>vote := (vote s) (a := (vote s a) (the (ballot s a) := suggestion s (the (ballot s a))))\<rparr>"
+              using a1 by metis
+            then have ff3: "vote t = (vote s) (a := (vote s a)(the (Some nn) := suggestion s (the (Some nn))))"
+              using ff1 by (metis p_state.select_convs(3) p_state.update_convs(3))
+            then have ff4: "vote t a = (vote s a)(the (Some nn) := suggestion s (the (Some nn)))"
+              by (metis fun_upd_apply)
+            then have ff5: "vote t a (the (Some nn)) = suggestion s (the (Some nn))"
+              by (metis fun_upd_apply)
+            have ff6: "\<And>aa. vote t aa = vote s aa \<or> a = aa"
+              using ff3 by (metis fun_upd_apply)
+            have "\<And>n. vote t a n = vote s a n \<or> the (Some nn) = n"
+              using ff4 by (metis fun_upd_apply)
+            then have "vote t aa b \<noteq> Some cc \<or> safe_at t (the (vote t aa b)) b"
+              using ff6 ff5 ff2 a4 a3 a2 by (metis option.case_eq_if prems(2) safe_mono) }
+          then show "let z = vote t aa b in (\<exists>c. z = Some c) \<longrightarrow> safe_at t (the z) b"
+            by metis
+        qed
+        from 1 2 3 safe_mono show ?thesis 
+          by (auto simp add:inv2_def)
+            (metis inv2_def option.case_eq_if prems(1) prems(2))
+      qed
+    subgoal premises prems for s t act b a
+    proof -
+      from prems(2,5) have 1:"join_ballot a b s t"
+        by(auto simp add:inv_proofs_defs)
+      hence 2:"\<And> b . suggestion s b = suggestion t b" 
+        by (auto simp add:inv_proofs_defs)
+      have 3:"safe t" using prems(1) 1 by (auto simp add:inv2_def safe_def) (metis prems(2) safe_mono)
+      from 1 2 3 safe_mono show ?thesis 
+        by (auto simp add:inv2_def)
+          (metis inv2_def option.case_eq_if prems(1) prems(2))
+    qed
+  subgoal premises prems for s t act b
+  proof -
+    from prems(2,5) have 1:"start_ballot b s t"
+      by(auto simp add:inv_proofs_defs)
+    have 3:"safe t" using prems(1) 1 by (auto simp add:inv2_def safe_def) (metis prems(2) safe_mono)
+    from 1 obtain q v where 2:"q |\<in>| quorums" and 4:"proved_safe_at s q b v" 
+      and 5:"t = s\<lparr>suggestion := suggestion s(b \<mapsto> v)\<rparr>" and 6:"\<And> a . a |\<in>| q \<Longrightarrow> ballot s a \<ge> Some b"
+      by auto
+    have 2:"\<And> b . case suggestion t b of None \<Rightarrow> True | Some v \<Rightarrow> safe_at t v b"
+      using 1 2 4 5 6 prems(1,2,3) apply(simp add:inv2_def)
+        by (metis option.case_eq_if proved_safe_is_safe safe_mono)
+    from 2 3 show ?thesis by (auto simp add:inv2_def)
+  qed
+done
+declare inv2[invs]
+
+lemma safe_inv:
+  "invariant the_ioa safe"
+apply(rule invariantI)
+    apply (force simp add:safe_def inv_proofs_defs)
+  apply instantiate_invs_2
+  apply (case_tac a)
+          apply (force simp add:safe_def inv_proofs_defs safe_at_def choosable_def)
+        apply (force simp add:safe_def inv_proofs_defs safe_at_def choosable_def)
+      apply (auto simp add:is_trans_def the_ioa_def p_ioa_def p_trans_def inv2_def)
+done
+declare safe_inv[invs]
+
+definition agreement where 
+  "agreement s \<equiv> \<forall> v w . chosen s v \<and> chosen s w \<longrightarrow> v = w"
+lemma "invariant the_ioa agreement"
+apply(rule invariantI)
+    apply(auto simp add: inv_proofs_defs agreement_def chosen_def chosen_at_def)[1]
+    apply (metis fempty_iff quorum_inter_witness)
+  apply instantiate_invs_2
+  apply (insert safe_is_safe)
+  apply (force simp add:agreement_def)
+done
 
 end
+
+subsection {* A mislead attempt at defining the max vote *}
+
+fun max_vote_2 where
+  "max_vote_2 votes (0::nat) = votes 0 \<bind> (\<lambda> v . Some (0,v))"
+| "max_vote_2 votes (Suc b) = 
+    ( case (votes (Suc b)) of None \<Rightarrow> max_vote_2 votes b
+      |  Some v \<Rightarrow> Some (Suc b, v) )"
+
+lemma assumes "i \<le> b" and "votes i \<noteq> None"
+  shows "case (max_vote_2 votes b) of None \<Rightarrow> False | Some (m,v) \<Rightarrow> i \<le> m"
+using assms
+proof (induct votes b rule:max_vote_2.induct)
+  case 1 thus ?case by fastforce
+next
+  case 2 thus ?case by auto (metis case_prodI le_Suc_eq option.case_eq_if option.sel option.simps(3))
+qed
+
+declare option.split[split]
+
+lemma
+  "case (max_vote_2 votes b) of None \<Rightarrow> True | Some (m,v) \<Rightarrow> m \<le> b \<and> votes m = Some v"
+proof (induct votes b rule:max_vote_2.induct)
+case (1 votes) thus ?case 
+  apply (auto)
+    apply (metis (no_types, lifting) Pair_inject bind_eq_Some_conv option.inject)
+  apply (smt bind_eq_Some_conv option.sel prod.inject)
+  done
+next
+  case (2 votes b) thus ?case by auto
+qed
 
 end
